ch15-dynamic-programming/CLRS.Ch15.RodCutting.Test.fst
@@ -10,7 +10,7 @@ module CLRS.Ch15.RodCutting.Test
 open Pulse.Lib.Pervasives
 open Pulse.Lib.Array
 open FStar.SizeT
-open CLRS.Ch15.RodCutting
+open CLRS.Ch15.RodCutting.Impl
 
 module A = Pulse.Lib.Array
 module V = Pulse.Lib.Vec
